src/goose_lang/interpreter/interpreter.v
@@ -869,6 +869,17 @@ Ltac runStateT_inv :=
         single_step.
         exact H.
       }
+      { runStateT_inv.
+        destruct v2 eqn:?; simpl in H; try by inversion H.
+        destruct l2 eqn:?; simpl in H; try by inversion H.
+        subst.
+        Transitions.monad_inv.
+        do 2 eexists.
+        eapply nsteps_transitive; [ctx_step (fill [(Primitive2LCtx AtomicStoreOp e2)])|].
+        eapply nsteps_transitive; [ctx_step (fill [(Primitive2RCtx AtomicStoreOp #l4)])|].
+        single_step.
+        exact H.
+      }
     }
 
     (* CmpXchg *)
